Notations.v
@@ -5,14 +5,13 @@ From Coq Require Import Strings.String.
 
 
 Declare Scope utils_scope.
-(* Delimit Scope utils_scope with utils. *)
+Delimit Scope utils_scope with utils.
 
 Notation "X ⇀ Y" :=  (X -> option Y) (at level 100): type_scope.
-Notation "A '^*'" := (list A) (at level 20) : type_scope.
+Notation "A ⃰" := (list A) (at level 20) : type_scope.
 
 Declare Custom Entry pmap.
 Reserved Notation "⊥".
-Reserved Notation "f { x \ y }" (at level 10).
 Reserved Notation "'dom' f" (at level 10).
 Notation "x '\' y" := (x,y) (in custom pmap at level 0, x constr, y constr) : utils_scope.
 Reserved Notation "f { xy , .. , xy' }" (xy custom pmap, xy' custom pmap, at level 0).
